Transfer network fairness accross stutter, match

fairneris/aneris_lang/network_model.v
@@ -1,7 +1,6 @@
 From trillium.prelude Require Export finitary quantifiers sigma classical_instances.
-From fairneris Require Export trace_utils fairness env_model fuel.
+From fairneris Require Export trace_utils fairness env_model fuel ltl_lite.
 From fairneris.aneris_lang Require Import ast network lang aneris_lang.
-
 
 Definition net_state : Set :=
   message_multi_soup * gmap socket_address (list message).
@@ -30,14 +29,6 @@ Program Definition net_lts : Lts (action aneris_lang + config_label aneris_lang)
     lts_state := net_state;
     lts_trans := net_trans;
   |}.
-
-Record Lts lab `{Countable lab, Inhabited lab}: Type := {
-  lts_state :> Type;
-  lts_state_eqdec :: EqDecision lts_state;
-  lts_state_inhabited :: Inhabited lts_state;
-
-  lts_trans: lts_state → lab → lts_state → Prop;
-}.
 
 Definition model_state_socket_coh
            (skts : gmap ip_address sockets)
@@ -82,8 +73,120 @@ Next Obligation.
   (* Unlabeled steps don't change the network state *)
 Admitted.
 
-Class LiveModelEq `(LM: LiveModel aneris_lang (joint_model Mod network_model)) := {
+Class LiveModelEq `(LM: LiveModel aneris_lang (joint_model Mod net_model)) := {
     cfg_labels_match_is_eq: ∀ x y, lm_cfg_labels_match LM x y ↔ x = y;
     actions_match_is_eq: ∀ x y, lm_actions_match LM x y ↔ Some x = y;
 }.
-Arguments LiveModelEq {_ _}.
+Arguments LiveModelEq {_}.
+
+Section fairness.
+  Context {M: UserModel aneris_lang}.
+
+  Notation jmlabel := ((usr_role M * option (action aneris_lang)) + config_label aneris_lang)%type.
+  Notation jmtrace := (trace (joint_model M net_model) jmlabel).
+
+  Definition send_filter msg : jmlabel → Prop :=
+    λ l, ∃ ρ, l = inl $ (ρ, Some $ Send msg).
+  Instance send_filter_decision msg l : Decision (send_filter msg l).
+  Proof. apply make_decision. Qed.
+
+  Definition deliver_filter msg : jmlabel → Prop :=
+    λ l, l = inr $ Deliver msg.
+  Instance deliver_filter_decision msg l : Decision (deliver_filter msg l).
+  Proof. apply make_decision. Qed.
+
+  Definition network_fair_delivery_of msg : jmtrace → Prop :=
+    □ (□◊ ℓ↓send_filter msg → ◊ ℓ↓ deliver_filter msg).
+
+  Definition network_fair_delivery (mtr : jmtrace) : Prop :=
+    ∀ msg, network_fair_delivery_of msg mtr.
+End fairness.
+
+Section fuel_fairness.
+  Context `{@LiveModelEq M LM}.
+
+  Notation jmlabel := ((usr_role M * option (action aneris_lang)) + config_label aneris_lang)%type.
+  Notation jmtrace := (trace (joint_model M net_model) jmlabel).
+
+  Notation fuel_trace := (trace LM LM.(lm_lbl)).
+
+  Definition fuel_send_filter msg : LM.(lm_lbl) → Prop :=
+    λ l, ∃ ρ ζ x, l = Take_step ρ (Some $ Send msg : fmaction (joint_model M _)) ζ x.
+  Instance fuel_send_filter_decision msg l : Decision (fuel_send_filter msg l).
+  Proof. apply make_decision. Qed.
+
+  Definition fuel_deliver_filter msg : LM.(lm_lbl) → Prop :=
+    λ l, ∃ x, l = Config_step (Deliver msg : fmconfig (joint_model M _)) x.
+  Instance fuel_deliver_filter_decision msg l : Decision (fuel_deliver_filter msg l).
+  Proof. apply make_decision. Qed.
+
+  Definition fuel_network_fair_delivery_of msg : fuel_trace → Prop :=
+    □ (□◊ ℓ↓fuel_send_filter msg → ◊ ℓ↓ fuel_deliver_filter msg).
+
+  Definition fuel_network_fair_delivery (mtr : fuel_trace) : Prop :=
+    ∀ msg, fuel_network_fair_delivery_of msg mtr.
+
+  Lemma fuel_network_fairness_destutter :
+    fuel_se fuel_network_fair_delivery network_fair_delivery.
+  Proof.
+    apply ltl_se_forall=> msg.
+    apply ltl_se_always, ltl_se_impl.
+    - apply ltl_se_always, ltl_se_eventually_now.
+      intros l. rewrite /fuel_send_filter /send_filter. split.
+      + intros (?&?&?). simplify_eq. naive_solver.
+      + intros (?&?&?&?). simplify_eq. destruct l=>//. simpl in *. simplify_eq.
+        eexists _, _, _. reflexivity.
+    - apply ltl_se_eventually_now.
+      intros l. rewrite /fuel_deliver_filter /deliver_filter. split; first naive_solver.
+      + intros (?&?&?). simplify_eq. destruct l=>//. simpl in *; simplify_eq. naive_solver.
+  Qed.
+End fuel_fairness.
+
+Eval cbv in (ex_label aneris_lang).
+
+Definition ex_send_filter msg : ex_label aneris_lang → Prop :=
+  λ l, sum_map snd id l = inl $ Some $ Send msg.
+Instance ex_send_filter_decision msg l : Decision (ex_send_filter msg l).
+Proof. apply make_decision. Qed.
+
+Definition ex_deliver_filter msg : ex_label aneris_lang → Prop :=
+  λ l, sum_map snd id l = inr $ Deliver msg.
+Instance ex_deliver_filter_decision msg l : Decision (ex_deliver_filter msg l).
+Proof. apply make_decision. Qed.
+Definition ex_fair_network_of msg : extrace aneris_lang → Prop :=
+  □ (□◊ ℓ↓ex_send_filter msg → ◊ ℓ↓ex_deliver_filter msg).
+
+Definition ex_fair_network (extr : extrace aneris_lang) : Prop :=
+  ∀ msg, ex_fair_network_of msg extr.
+
+Section exec_fairness.
+  Context `{@LiveModelEq M LM}.
+
+  Lemma exec_fuel_fairness:
+    exaux_tme (LM := LM) ex_fair_network fuel_network_fair_delivery.
+  Proof.
+    apply ltl_tme_forall=> msg.
+    apply ltl_tme_always, ltl_tme_impl.
+    - apply ltl_tme_always, ltl_tme_eventually, ltl_tme_now.
+      intros l1 l2 Hlm. split.
+      + destruct l1 as [[? [|]]|], l2 =>//=; try naive_solver.
+        rewrite /ex_send_filter /=. intros ?. simplify_eq.
+        destruct Hlm as (?&?&Hlm). apply actions_match_is_eq in Hlm. simplify_eq.
+        rewrite /fuel_send_filter. naive_solver.
+      + rewrite /fuel_send_filter /ex_send_filter.
+        destruct l1 as [[? [|]]|], l2 =>//=; try naive_solver.
+        intros ?. simplify_eq.
+        destruct Hlm as (?&?&Hlm). apply actions_match_is_eq in Hlm. simplify_eq.
+        rewrite /fuel_send_filter. naive_solver.
+    - apply ltl_tme_eventually, ltl_tme_now.
+      intros l1 l2 Hlm. split.
+      + destruct l1 as [|[| |]], l2 =>//=; try naive_solver.
+        rewrite /ex_deliver_filter /=. intros ?. simplify_eq.
+        destruct Hlm as (?&Hcm). apply cfg_labels_match_is_eq in Hcm. simplify_eq.
+        rewrite /fuel_deliver_filter. naive_solver.
+      + rewrite /ex_deliver_filter /fuel_deliver_filter. intros (?&?). simplify_eq.
+        destruct l1 as [[?[|]]|] =>//=; try naive_solver.
+        destruct Hlm as [? Hlm].
+        apply cfg_labels_match_is_eq in Hlm. simplify_eq. done.
+  Qed.
+End exec_fairness.
